src/Init/Data/Array/MapIdx.lean
@@ -5,6 +5,7 @@ Authors: Mario Carneiro, Kim Morrison
 -/
 prelude
 import Init.Data.Array.Lemmas
+import Init.Data.Array.Attach
 import Init.Data.List.MapIdx
 
 namespace Array
@@ -111,3 +112,293 @@ namespace List
   ext <;> simp
 
 end List
+
+namespace Array
+
+/-! ### zipWithIndex -/
+
+@[simp] theorem getElem_zipWithIndex (a : Array α) (i : Nat) (h : i < a.zipWithIndex.size) :
+    (a.zipWithIndex)[i] = (a[i]'(by simp_all), i) := by
+  simp [zipWithIndex]
+
+@[simp] theorem zipWithIndex_toArray {l : List α} :
+    l.toArray.zipWithIndex = (l.enum.map fun (i, x) => (x, i)).toArray := by
+  ext i hi₁ hi₂ <;> simp
+
+@[simp] theorem toList_zipWithIndex (a : Array α) :
+    a.zipWithIndex.toList = a.toList.enum.map (fun (i, a) => (a, i)) := by
+  rcases a with ⟨a⟩
+  simp
+
+theorem mk_mem_zipWithIndex_iff_getElem? {x : α} {i : Nat} {l : Array α} :
+    (x, i) ∈ l.zipWithIndex ↔ l[i]? = x := by
+  rcases l with ⟨l⟩
+  simp only [zipWithIndex_toArray, mem_toArray, List.mem_map, Prod.mk.injEq, Prod.exists,
+    List.mk_mem_enum_iff_getElem?, List.getElem?_toArray]
+  constructor
+  · rintro ⟨a, b, h, rfl, rfl⟩
+    exact h
+  · intro h
+    exact ⟨i, x, by simp [h]⟩
+
+theorem mem_enum_iff_getElem? {x : α × Nat} {l : Array α} : x ∈ l.zipWithIndex ↔ l[x.2]? = some x.1 :=
+  mk_mem_zipWithIndex_iff_getElem?
+
+/-! ### mapFinIdx -/
+
+@[congr] theorem mapFinIdx_congr {xs ys : Array α} (w : xs = ys)
+    (f : (i : Nat) → α → (h : i < xs.size) → β) :
+    mapFinIdx xs f = mapFinIdx ys (fun i a h => f i a (by simp [w]; omega)) := by
+  subst w
+  rfl
+
+@[simp]
+theorem mapFinIdx_empty {f : (i : Nat) → α → (h : i < 0) → β} : mapFinIdx #[] f = #[] :=
+  rfl
+
+theorem mapFinIdx_eq_ofFn {as : Array α} {f : (i : Nat) → α → (h : i < as.size) → β} :
+    as.mapFinIdx f = Array.ofFn fun i : Fin as.size => f i as[i] i.2 := by
+  cases as
+  simp [List.mapFinIdx_eq_ofFn]
+
+theorem mapFinIdx_append {K L : Array α} {f : (i : Nat) → α → (h : i < (K ++ L).size) → β} :
+    (K ++ L).mapFinIdx f =
+      K.mapFinIdx (fun i a h => f i a (by simp; omega)) ++
+        L.mapFinIdx (fun i a h => f (i + K.size) a (by simp; omega)) := by
+  cases K
+  cases L
+  simp [List.mapFinIdx_append]
+
+@[simp]
+theorem mapFinIdx_push {l : Array α} {a : α} {f : (i : Nat) → α → (h : i < (l.push a).size) → β} :
+    mapFinIdx (l.push a) f =
+      (mapFinIdx l (fun i a h => f i a (by simp; omega))).push (f l.size a (by simp)) := by
+  simp [← append_singleton, mapFinIdx_append]
+
+theorem mapFinIdx_singleton {a : α} {f : (i : Nat) → α → (h : i < 1) → β} :
+    #[a].mapFinIdx f = #[f 0 a (by simp)] := by
+  simp
+
+theorem mapFinIdx_eq_zipWithIndex_map {l : Array α} {f : (i : Nat) → α → (h : i < l.size) → β} :
+    l.mapFinIdx f = l.zipWithIndex.attach.map
+      fun ⟨⟨x, i⟩, m⟩ =>
+        f i x (by simp [mk_mem_zipWithIndex_iff_getElem?, getElem?_eq_some_iff] at m; exact m.1) := by
+  ext <;> simp
+
+@[simp]
+theorem mapFinIdx_eq_empty_iff {l : Array α} {f : (i : Nat) → α → (h : i < l.size) → β} :
+    l.mapFinIdx f = #[] ↔ l = #[] := by
+  cases l
+  simp
+
+theorem mapFinIdx_ne_empty_iff {l : Array α} {f : (i : Nat) → α → (h : i < l.size) → β} :
+    l.mapFinIdx f ≠ #[] ↔ l ≠ #[] := by
+  simp
+
+theorem exists_of_mem_mapFinIdx {b : β} {l : Array α} {f : (i : Nat) → α → (h : i < l.size) → β}
+    (h : b ∈ l.mapFinIdx f) : ∃ (i : Nat) (h : i < l.size), f i l[i] h = b := by
+  rcases l with ⟨l⟩
+  exact List.exists_of_mem_mapFinIdx (by simpa using h)
+
+@[simp] theorem mem_mapFinIdx {b : β} {l : Array α} {f : (i : Nat) → α → (h : i < l.size) → β} :
+    b ∈ l.mapFinIdx f ↔ ∃ (i : Nat) (h : i < l.size), f i l[i] h = b := by
+  rcases l with ⟨l⟩
+  simp
+
+theorem mapFinIdx_eq_iff {l : Array α} {f : (i : Nat) → α → (h : i < l.size) → β} :
+    l.mapFinIdx f = l' ↔ ∃ h : l'.size = l.size, ∀ (i : Nat) (h : i < l.size), l'[i] = f i l[i] h := by
+  rcases l with ⟨l⟩
+  rcases l' with ⟨l'⟩
+  simpa using List.mapFinIdx_eq_iff
+
+@[simp] theorem mapFinIdx_eq_singleton_iff {l : Array α} {f : (i : Nat) → α → (h : i < l.size) → β} {b : β} :
+    l.mapFinIdx f = #[b] ↔ ∃ (a : α) (w : l = #[a]), f 0 a (by simp [w]) = b := by
+  rcases l with ⟨l⟩
+  simp
+
+theorem mapFinIdx_eq_append_iff {l : Array α} {f : (i : Nat) → α → (h : i < l.size) → β} {l₁ l₂ : Array β} :
+    l.mapFinIdx f = l₁ ++ l₂ ↔
+      ∃ (l₁' : Array α) (l₂' : Array α) (w : l = l₁' ++ l₂'),
+        l₁'.mapFinIdx (fun i a h => f i a (by simp [w]; omega)) = l₁ ∧
+        l₂'.mapFinIdx (fun i a h => f (i + l₁'.size) a (by simp [w]; omega)) = l₂ := by
+  rcases l with ⟨l⟩
+  rcases l₁ with ⟨l₁⟩
+  rcases l₂ with ⟨l₂⟩
+  simp only [List.mapFinIdx_toArray, List.append_toArray, mk.injEq, List.mapFinIdx_eq_append_iff,
+    toArray_eq_append_iff]
+  constructor
+  · rintro ⟨l₁, l₂, rfl, rfl, rfl⟩
+    refine ⟨l₁.toArray, l₂.toArray, by simp_all⟩
+  · rintro ⟨⟨l₁⟩, ⟨l₂⟩, rfl, h₁, h₂⟩
+    simp [← toList_inj] at h₁ h₂
+    obtain rfl := h₁
+    obtain rfl := h₂
+    refine ⟨l₁, l₂, by simp_all⟩
+
+theorem mapFinIdx_eq_push_iff {l : Array α} {b : β} {f : (i : Nat) → α → (h : i < l.size) → β} :
+    l.mapFinIdx f = l₂.push b ↔
+      ∃ (l₁ : Array α) (a : α) (w : l = l₁.push a),
+        l₁.mapFinIdx (fun i a h => f i a (by simp [w]; omega)) = l₂ ∧ b = f (l.size - 1) a (by simp [w]) := by
+  rw [push_eq_append, mapFinIdx_eq_append_iff]
+  constructor
+  · rintro ⟨l₁, l₂, rfl, rfl, h₂⟩
+    simp only [mapFinIdx_eq_singleton_iff, Nat.zero_add] at h₂
+    obtain ⟨a, rfl, rfl⟩ := h₂
+    exact ⟨l₁, a, by simp⟩
+  · rintro ⟨l₁, a, rfl, rfl, rfl⟩
+    exact ⟨l₁, #[a], by simp⟩
+
+theorem mapFinIdx_eq_mapFinIdx_iff {l : Array α} {f g : (i : Nat) → α → (h : i < l.size) → β} :
+    l.mapFinIdx f = l.mapFinIdx g ↔ ∀ (i : Nat) (h : i < l.size), f i l[i] h = g i l[i] h := by
+  rw [eq_comm, mapFinIdx_eq_iff]
+  simp
+
+@[simp] theorem mapFinIdx_mapFinIdx {l : Array α}
+    {f : (i : Nat) → α → (h : i < l.size) → β}
+    {g : (i : Nat) → β → (h : i < (l.mapFinIdx f).size) → γ} :
+    (l.mapFinIdx f).mapFinIdx g = l.mapFinIdx (fun i a h => g i (f i a h) (by simpa using h)) := by
+  simp [mapFinIdx_eq_iff]
+
+theorem mapFinIdx_eq_mkArray_iff {l : Array α} {f : (i : Nat) → α → (h : i < l.size) → β} {b : β} :
+    l.mapFinIdx f = mkArray l.size b ↔ ∀ (i : Nat) (h : i < l.size), f i l[i] h = b := by
+  rcases l with ⟨l⟩
+  rw [← toList_inj]
+  simp [List.mapFinIdx_eq_replicate_iff]
+
+@[simp] theorem mapFinIdx_reverse {l : Array α} {f : (i : Nat) → α → (h : i < l.reverse.size) → β} :
+    l.reverse.mapFinIdx f = (l.mapFinIdx (fun i a h => f (l.size - 1 - i) a (by simp; omega))).reverse := by
+  rcases l with ⟨l⟩
+  simp [List.mapFinIdx_reverse]
+
+/-! ### mapIdx -/
+
+@[simp]
+theorem mapIdx_empty {f : Nat → α → β} : mapIdx f #[] = #[] :=
+  rfl
+
+@[simp] theorem mapFinIdx_eq_mapIdx {l : Array α} {f : (i : Nat) → α → (h : i < l.size) → β} {g : Nat → α → β}
+    (h : ∀ (i : Nat) (h : i < l.size), f i l[i] h = g i l[i]) :
+    l.mapFinIdx f = l.mapIdx g := by
+  simp_all [mapFinIdx_eq_iff]
+
+theorem mapIdx_eq_mapFinIdx {l : Array α} {f : Nat → α → β} :
+    l.mapIdx f = l.mapFinIdx (fun i a _ => f i a) := by
+  simp [mapFinIdx_eq_mapIdx]
+
+theorem mapIdx_eq_zipWithIndex_map {l : Array α} {f : Nat → α → β} :
+    l.mapIdx f = l.zipWithIndex.map fun ⟨a, i⟩ => f i a := by
+  ext <;> simp
+
+theorem mapIdx_append {K L : Array α} :
+    (K ++ L).mapIdx f = K.mapIdx f ++ L.mapIdx fun i => f (i + K.size) := by
+  rcases K with ⟨K⟩
+  rcases L with ⟨L⟩
+  simp [List.mapIdx_append]
+
+@[simp]
+theorem mapIdx_push {l : Array α} {a : α} :
+    mapIdx f (l.push a) = (mapIdx f l).push (f l.size a) := by
+  simp [← append_singleton, mapIdx_append]
+
+theorem mapIdx_singleton {a : α} : mapIdx f #[a] = #[f 0 a] := by
+  simp
+
+@[simp]
+theorem mapIdx_eq_empty_iff {l : Array α} : mapIdx f l = #[] ↔ l = #[] := by
+  rcases l with ⟨l⟩
+  simp
+
+theorem mapIdx_ne_empty_iff {l : Array α} :
+    mapIdx f l ≠ #[] ↔ l ≠ #[] := by
+  simp
+
+theorem exists_of_mem_mapIdx {b : β} {l : Array α}
+    (h : b ∈ mapIdx f l) : ∃ (i : Nat) (h : i < l.size), f i l[i] = b := by
+  rw [mapIdx_eq_mapFinIdx] at h
+  simpa [Fin.exists_iff] using exists_of_mem_mapFinIdx h
+
+@[simp] theorem mem_mapIdx {b : β} {l : Array α} :
+    b ∈ mapIdx f l ↔ ∃ (i : Nat) (h : i < l.size), f i l[i] = b := by
+  constructor
+  · intro h
+    exact exists_of_mem_mapIdx h
+  · rintro ⟨i, h, rfl⟩
+    rw [mem_iff_getElem]
+    exact ⟨i, by simpa using h, by simp⟩
+
+theorem mapIdx_eq_push_iff {l : Array α} {b : β} :
+    mapIdx f l = l₂.push b ↔
+      ∃ (a : α) (l₁ : Array α), l = l₁.push a ∧ mapIdx f l₁ = l₂ ∧ f l₁.size a = b := by
+  rw [mapIdx_eq_mapFinIdx, mapFinIdx_eq_push_iff]
+  simp only [mapFinIdx_eq_mapIdx, exists_and_left, exists_prop]
+  constructor
+  · rintro ⟨l₁, rfl, a, rfl, rfl⟩
+    exact ⟨a, l₁, by simp⟩
+  · rintro ⟨a, l₁, rfl, rfl, rfl⟩
+    exact ⟨l₁, rfl, a, by simp⟩
+
+@[simp] theorem mapIdx_eq_singleton_iff {l : Array α} {f : Nat → α → β} {b : β} :
+    mapIdx f l = #[b] ↔ ∃ (a : α), l = #[a] ∧ f 0 a = b := by
+  rcases l with ⟨l⟩
+  simp [List.mapIdx_eq_singleton_iff]
+
+theorem mapIdx_eq_append_iff {l : Array α} {f : Nat → α → β} {l₁ l₂ : Array β} :
+    mapIdx f l = l₁ ++ l₂ ↔
+      ∃ (l₁' : Array α) (l₂' : Array α), l = l₁' ++ l₂' ∧
+        l₁'.mapIdx f = l₁ ∧
+        l₂'.mapIdx (fun i => f (i + l₁'.size)) = l₂ := by
+  rcases l with ⟨l⟩
+  rcases l₁ with ⟨l₁⟩
+  rcases l₂ with ⟨l₂⟩
+  simp only [List.mapIdx_toArray, List.append_toArray, mk.injEq, List.mapIdx_eq_append_iff,
+    toArray_eq_append_iff]
+  constructor
+  · rintro ⟨l₁, l₂, rfl, rfl, rfl⟩
+    exact ⟨l₁.toArray, l₂.toArray, by simp⟩
+  · rintro ⟨⟨l₁⟩, ⟨l₂⟩, rfl, h₁, h₂⟩
+    simp only [List.mapIdx_toArray, mk.injEq, size_toArray] at h₁ h₂
+    obtain rfl := h₁
+    obtain rfl := h₂
+    exact ⟨l₁, l₂, by simp⟩
+
+theorem mapIdx_eq_iff {l : Array α} : mapIdx f l = l' ↔ ∀ i : Nat, l'[i]? = l[i]?.map (f i) := by
+  rcases l with ⟨l⟩
+  rcases l' with ⟨l'⟩
+  simp [List.mapIdx_eq_iff]
+
+theorem mapIdx_eq_mapIdx_iff {l : Array α} :
+    mapIdx f l = mapIdx g l ↔ ∀ i : Nat, (h : i < l.size) → f i l[i] = g i l[i] := by
+  rcases l with ⟨l⟩
+  simp [List.mapIdx_eq_mapIdx_iff]
+
+@[simp] theorem mapIdx_set {l : Array α} {i : Nat} {h : i < l.size} {a : α} :
+    (l.set i a).mapIdx f = (l.mapIdx f).set i (f i a) (by simpa) := by
+  rcases l with ⟨l⟩
+  simp [List.mapIdx_set]
+
+@[simp] theorem mapIdx_setIfInBounds {l : Array α} {i : Nat} {a : α} :
+    (l.setIfInBounds i a).mapIdx f = (l.mapIdx f).setIfInBounds i (f i a) := by
+  rcases l with ⟨l⟩
+  simp [List.mapIdx_set]
+
+@[simp] theorem back?_mapIdx {l : Array α} {f : Nat → α → β} :
+    (mapIdx f l).back? = (l.back?).map (f (l.size - 1)) := by
+  rcases l with ⟨l⟩
+  simp [List.getLast?_mapIdx]
+
+@[simp] theorem mapIdx_mapIdx {l : Array α} {f : Nat → α → β} {g : Nat → β → γ} :
+    (l.mapIdx f).mapIdx g = l.mapIdx (fun i => g i ∘ f i) := by
+  simp [mapIdx_eq_iff]
+
+theorem mapIdx_eq_mkArray_iff {l : Array α} {f : Nat → α → β} {b : β} :
+    mapIdx f l = mkArray l.size b ↔ ∀ (i : Nat) (h : i < l.size), f i l[i] = b := by
+  rcases l with ⟨l⟩
+  rw [← toList_inj]
+  simp [List.mapIdx_eq_replicate_iff]
+
+@[simp] theorem mapIdx_reverse {l : Array α} {f : Nat → α → β} :
+    l.reverse.mapIdx f = (mapIdx (fun i => f (l.size - 1 - i)) l).reverse := by
+  rcases l with ⟨l⟩
+  simp [List.mapIdx_reverse]
+
+end Array
